theories/tree_valid_cut.v
@@ -19,7 +19,7 @@ Fixpoint vars_tree t : {fset V} :=
   | x :: xs =>  *)
   
 
-Definition disj_tree T1 T2 := [disjoint (vars_tree T1) & (vars_tree T2)].
+Definition disj_tree T1 T2 := (vars_tree T1) `&` (vars_tree T2) == fset0.
 
 Set Implicit Arguments.
 Unset Strict Implicit.
@@ -54,8 +54,9 @@ Section valid_tree.
   Fixpoint base_or_aux s :=
     match s with
     | Or l _ r => 
-      (* [&& disj_tree l r, base_and l & (base_or_aux r)] todo: should also say something about the substitution and the program? *)
-      [&& base_and l & (base_or_aux r)] (* todo: should also say something about the substitution and the program? *)
+      (*todo: should also say something about the substitution and the program? *)
+      [&& disj_tree l r, base_and l & (base_or_aux r)] 
+      (* [&& base_and l & (base_or_aux r)] todo: should also say something about the substitution and the program? *)
     | t => base_and t
     end.
 
@@ -88,17 +89,28 @@ Section valid_tree.
   Lemma check_cut_refl A: check_cut A A.
   Proof. rewrite/check_cut; case: ifP => ->; rewrite ?orbT//. Qed.
 
+  Fixpoint resetR' B0 B :=
+    match B0, B with
+    | OK, OK => true
+    | And L1 _ R1, And L2 _ R2 =>
+      if L1 == L2 then R1 == R2
+      else disj_tree L1 L2 && resetR' R1 R2
+    | _, _ => false
+    end.
+
+  Definition resetR B0 B := (is_ko B0 || resetR' B0 B).
+
   Fixpoint valid_tree s :=
     match s with
     | CutS | CallS _ _ | OK | Bot => true
     | Dead => false
     | Or A _ B =>
-      (*disj_tree A B &&*)
+      disj_tree A B &&
       if is_dead A then valid_tree B
       else valid_tree A && (bbOr B)
     | And A B0 B => 
       [&& valid_tree A,
-        if success A then valid_tree B 
+        if success A then (valid_tree B (*&& resetR B0 B*))
         else (B0 == B),
         (if success A || failed A then bbAnd B0 else base_and B0)
         & check_cut B B0]
@@ -154,22 +166,106 @@ Section valid_tree.
   Lemma big_or_aux_not_bot {pr l rs}: big_or_aux pr l rs != Bot.
   Proof. case: rs => [|[] xs]//=; case: l => //. Qed.
 
-  Lemma bbOr_big_or_aux {pr s l}: bbOr (big_or_aux pr s l).
+  Lemma vars_big_and pr r1:
+    vars_tree (big_and pr r1) = varsU (map vars_atom r1).
   Proof.
-    rewrite/bbOr.
-    case: base_or_aux_ko; rewrite ?orbT//orbF.
+    elim: r1 => //= x xs IH; rewrite IH//.
+    rewrite -fsetUA fsetUid.
+    destruct x => //.
+  Qed.
+
+  Lemma vars_big_or_aux pr r rs:
+    vars_tree (big_or_aux pr r rs) = 
+      varsU (map vars_atom r) `|` varsU [seq varsU_rprem x.2 | x <- rs].
+  Proof. by elim: rs r => //=[|[s r] rs IH] r1/=; rewrite vars_big_and ?fsetU0// IH. Qed.
+
+  Lemma bbOr_big_or_aux {pr s l}:
+    varsD (varsU (map vars_atom s) :: ((map (fun x => varsU_rprem x.2) l))) ->
+    bbOr (big_or_aux pr s l).
+  Proof.
+    rewrite/bbOr => /=/andP[].
+    case: base_or_aux_ko; rewrite ?orbT//orbF/=.
     elim: l s => //=; clear.
     + move=> []//a l; rewrite /base_or_aux //= base_and_big_and eqxx//.
       case: a => //.
-    + by move=> [s r] rs IH r1 /=; rewrite IH base_and_big_and.
+    + move=> [s r] rs IH r1 /=.
+      rewrite !fsetIUr !fsetU_eq0.
+      move=> /andP[H1 H2] /andP[H4 H5].
+      rewrite base_and_big_and/= IH//=.
+      rewrite/disj_tree.
+      rewrite vars_big_and vars_big_or_aux.
+      by rewrite !fsetIUr !fsetU_eq0 H1 H2.
+  Qed.
+
+  Definition is_base s := match s with 
+    | Bot | Dead | OK | CutS => true 
+    | Or _ _ _ | And _ _ _ | CallS _ _ => false
+    end.
+
+  Lemma disj_tree_baseL b r: is_base b -> disj_tree b r.
+  Proof. by destruct b; rewrite ///disj_tree/= fset0I. Qed.
+
+  Hint Resolve disj_tree_baseL : core.
+
+  Lemma disj_tree_commE A B: disj_tree A B = disj_tree B A.
+  Proof. by rewrite/disj_tree fsetIC. Qed.
+
+  Lemma disj_tree_comm A B: disj_tree A B -> disj_tree B A.
+  Proof. by rewrite disj_tree_commE. Qed.
+
+  Lemma disj_tree_AndE A B C D:
+    disj_tree (And A B C) D = disj_tree A D && disj_tree B D && disj_tree C D.
+  Proof. by rewrite/disj_tree /= !fsetIUl !fsetU_eq0. Qed.
+
+  Lemma disj_tree_And A B C D:
+    [/\ disj_tree A D, disj_tree B D & disj_tree C D] <-> disj_tree (And A B C) D.
+  Proof. by rewrite disj_tree_AndE; split => [[]|/andP[/andP[]]]->->->. Qed.
+
+  Lemma disj_tree_OrE A s B C:
+    disj_tree (Or A s B) C = disj_tree A C && disj_tree B C.
+  Proof. by rewrite/disj_tree /= !fsetIUl !fsetU_eq0. Qed.
+
+  Lemma disj_tree_Or A s B C:
+    (disj_tree A C /\ disj_tree B C) <-> disj_tree (Or A s B) C.
+  Proof. rewrite disj_tree_OrE//; split => [[]|/andP[]]->->//. Qed.
+
+  Lemma disj_tree_cutrL A C: disj_tree (cutr A) C.
+  Proof.
+    elim: A => /=; only 1-5: by rewrite disj_tree_baseL.
+      by move=> A HA s B HB; apply/disj_tree_Or; rewrite HA HB.
+    by move=> A HA B0 HB0 B HB; apply/ disj_tree_And; rewrite HA HB HB0.
+  Qed.
+
+  Lemma disj_tree_cutrR A C: disj_tree C (cutr A).
+  Proof. apply: disj_tree_comm (disj_tree_cutrL _ _). Qed.
+
+  Lemma disj_tree_cutlL A C: disj_tree A C -> disj_tree (cutl A) C.
+  Proof.
+    elim: A => //=; first by rewrite disj_tree_baseL.
+      move=> A HA s B HB /disj_tree_Or[dAC dBC];
+      case: ifP => dA; apply/disj_tree_Or; split; auto;
+      apply: disj_tree_cutrL.
+    move=> A HA B0 HB0 B HB/disj_tree_And[dA dB0 dB];
+    case: ifP => _; apply/disj_tree_And; split; auto;
+    apply: disj_tree_cutrL.
+  Qed.
+
+  Lemma disj_tree_cutlR A C: disj_tree A C -> disj_tree A (cutl C).
+  Proof. by move=> H; apply/disj_tree_comm/disj_tree_cutlL/disj_tree_comm. Qed.
+
+  Lemma disj_tree_deadL A C: disj_tree (dead A) C.
+  Proof.
+    elim: A => /=; only 1-5: by rewrite disj_tree_baseL.
+      move=> A HA s B HB; apply/ disj_tree_Or; split; auto.
+    by move=> A HA B0 HB0 B HB; apply/ disj_tree_And; split.
   Qed.
 
   Lemma valid_tree_big_or {pr s t} : valid_tree (big_or u pr s t).
   Proof.
-    case: t; rewrite /big_or//=.
-    + move=> c; case: F => // -[] //s1 r rs/=; rewrite bbOr_big_or_aux//.
-    + move=> c; case: F => // -[] //s1 r rs/=; rewrite bbOr_big_or_aux//.
-    + move=> ??; case: F => // -[] //s1 r rs/=; rewrite bbOr_big_or_aux//. 
+    rewrite /big_or//=.
+    case: t => [k|v|c t]; case H: F => // [[s1 r] rs]; 
+    rewrite /=!(bbOr_big_or_aux,disj_tree_baseL)//;
+    apply: backchain_fresh_premE H.
   Qed.
 
   Lemma base_and_ko_valid {B}: base_and_ko B -> valid_tree B.
@@ -185,17 +281,25 @@ Section valid_tree.
   Lemma base_and_ko_base_or_aux_ko {A}: base_and_ko A -> base_or_aux_ko A.
   Proof. case: A => //. Qed.
 
+  Lemma base_and_ko_disj A C:
+    base_and_ko A -> disj_tree A C.
+  Proof.
+    elim: A => //; first by rewrite disj_tree_baseL//.
+    move=> []// _ _ _ B HB/= /and3P[_ /eqP->] => /HB{}HB.
+    apply/disj_tree_And; split => //; rewrite disj_tree_baseL//.
+  Qed.    
+
   Lemma bbOr_valid {B}:
     bbOr B -> valid_tree B.
   Proof. 
     move=> /orP [].
     elim B => //; clear.
-    + move=> A HA s B HB/=/andP[bA bB].
-      rewrite HA ?base_and_base_or_aux// /bbOr bB HB// if_same//base_and_is_and//orbT//.
+    + move=> A HA s B HB/=/and3P[dAB bA bB].
+      rewrite HA ?base_and_base_or_aux// /bbOr bB HB//dAB if_same//base_and_is_and//orbT//.
     + by move=> s; case: s => //[p t|] Ha B0 HB0 B HB /=/andP[/eqP->]bB; rewrite eqxx bB//check_cut_refl.
     elim: B => //.
     + move=> A HA s B HB /= /andP [bA bB].
-      rewrite HB//HA?base_and_ko_base_or_aux_ko// /bbOr bB orbT if_same//base_and_ko_is_and//orbT//.
+      rewrite HB//HA?base_and_ko_base_or_aux_ko// /bbOr bB orbT if_same//base_and_ko_disj//.
     + move=> [] // HA B0 _ B HB /= /and3P[] bB0 /eqP <-.
       by rewrite /bbAnd bB0 eqxx // orbT//check_cut_refl.
   Qed.
@@ -221,7 +325,7 @@ Section valid_tree.
   Lemma base_or_base_or_ko_cutr {B}: base_or_aux B -> base_or_aux_ko (cutr B).
   Proof.
     elim: B => //.
-    + move=> A IHA s B IHB /= /andP [] /base_and_base_and_ko_cutr -> /IHB ->//.
+    + move=> A IHA s B IHB /= /and3P[dAB] /base_and_base_and_ko_cutr -> /IHB ->//.
     + move=> a; case: a => //=[_ _|] _ B HB C HC /andP [] /eqP /[subst1] hC;
       rewrite base_and_base_and_ko_cutr//eqxx//.
   Qed.
@@ -281,30 +385,33 @@ Section valid_tree.
   Lemma has_cut_dead A: has_cut (dead A) = false.
   Proof. by elim: A => //=A -> B0 -> B ->. Qed.
 
-  Lemma valid_tree_cutr {A}: valid_tree A -> valid_tree (cutr A).
+  (* Lemma valid_tree_cutr {A}: valid_tree A -> valid_tree (cutr A).
   Proof.
     elim: A => //.
     - move=> A HA s B HB/=.
-      rewrite is_dead_cutr.
-      case: ifP => [dA vA|dA/andP[vA bB]]//; auto.
-      by rewrite bbOr_cutr//HA//.
+      rewrite is_dead_cutr disj_tree_cutrL.
+      case: ifP => [dA /andP[dAB vA]|dA/and3P[dAB vA bB]]//;
+      by rewrite !(HA, HB, bbOr_cutr)//.
     - move=> A HA B0 HB0 B HB/=/and4P[vA ++ C]; rewrite check_cut_cutrR/=.
-      case: ifP => /=[sA vB bB| sA /eqP -> bB].
+      case: ifP => /=[sA vB bB| sA /eqP -> bB];
+      rewrite !(HA, success_cutr, failed_cutr, bac)//=.
       rewrite?has_cut_cutr//=HA//HB//. 
         (* ?bbOr_valid// iscuc. *)
       (* rewrite HA//HB//bbAnd_cutr// success_cutr failed_cutr/=andbT. *)
-  Abort.
+  Abort. *)
+
+  Lemma resetR_cutrR B0 B: resetR (cutr B0) B.
+  Proof. rewrite/resetR is_ko_cutr//. Qed.
 
   Lemma valid_tree_cut {A}: success A -> valid_tree A -> valid_tree (cutl A).
   Proof.
     elim: A => //.
       move=> A HA s B HB => /=.
-      case: ifP => //[dA sB vB| dA sA /andP[vA bB]]/=.
-        rewrite dA HB//.
-      rewrite is_dead_cutl dA HA// bbOr_cutr//.
+      case: ifP => //[dA sB /andP[dAB vB]| dA sA /and3P[dAB vA bB]]/=;
+      rewrite !(dA, HB, HA,is_dead_cutl,bbOr_cutr,disj_tree_cutlR,disj_tree_cutrR)//.
     move=> A HA B0 HB0 B HB /= /andP[sA sB] /and4P[vA ++ C].
     rewrite sA/= => vB bB.
-    by rewrite success_cut sA HA//HB//=bbAnd_cutr// check_cut_cutrR.
+    rewrite success_cut sA HA//HB//=bbAnd_cutr// check_cut_cutrR//.
   Qed.
 
   Lemma base_and_bbAnd {A}: base_and A -> bbAnd A.
@@ -330,6 +437,142 @@ Section valid_tree.
     step u s A = r -> ~~(is_cutbrothers r) -> check_cut (get_tree r) B0 = check_cut A B0.
   Proof. by move=> eA H; rewrite/check_cut (step_keep_cut eA)//. Qed.
 
+  Lemma disj_tree_step s X B l: 
+    step u s B = l ->
+    disj_tree B X -> disj_tree (get_tree (l)) X.
+  Proof.
+    move=> <-{l}.
+    elim: B s => //=.
+    - move=> p c s H; rewrite/big_or.
+      case F: F => [|[s1 r] rs]; first by rewrite disj_tree_baseL.
+      apply/disj_tree_Or; split; first by apply:disj_tree_baseL.
+      move: H.
+      rewrite/disj_tree vars_big_or_aux/=.
+      move=> H.
+      (* move:H; rewrite/ditreq   *)
+
+       admit.
+    - move=> A HA s B HB s1 /disj_tree_Or[dA dB].
+      case:ifP => deadA.
+        have:= HB s dB; case step => /= B' {}HB;
+        by apply/disj_tree_Or; rewrite dA//.
+      have:= HA s1 dA; case: step => /= A' {}HA;
+      by apply/disj_tree_Or; split; rewrite//disj_tree_cutrL.
+    - move=> A HA B0 HB0 B HB s /disj_tree_And[dA dB0 dB].
+      have:= HA s dA; case: step => /= A' {}HA; 
+      only 1-3: by (apply/disj_tree_And; split).
+      by have:= HB (get_substS s A') dB; case: step => //=B' {}HB;
+      apply/disj_tree_And; split; auto; rewrite (disj_tree_cutlL,disj_tree_cutrL).
+  Admitted.
+
+  Lemma disj_tree_stepR s X B l: 
+    step u s B = l ->
+    disj_tree X B -> disj_tree X (get_tree (l)).
+  Proof. by move=> /disj_tree_step H /disj_tree_comm/H /disj_tree_comm. Qed.
+
+  Lemma base_and_ko_is_ko {A}: base_and_ko A -> is_ko A.
+  Proof. elim: A => //=-[]//. Qed.
+
+  Lemma base_and_failed {A}: base_and A -> failed A = false.
+  Proof. elim: A => //=-[]//=p a _ A HA B HB /andP[]//. Qed.
+
+  Lemma base_and_is_ko A: base_and A -> is_ko A = false.
+  Proof. move=> bA; rewrite failed_is_ko//base_and_failed//. Qed.
+
+  Lemma resetR_base_and_ko B0 C:
+    base_and_ko B0 -> resetR B0 C.
+  Proof. by rewrite/resetR; move=> /base_and_ko_is_ko->. Qed.
+
+  Definition is_call A := match A with CallS _ _ => true | _ => false end.
+
+  Lemma base_and_AndP A B0 B: base_and (And A B0 B) <-> 
+    [/\ (A = CutS \/ is_call A), (B0 = B) & base_and B].
+  Proof.
+    split => /=; first by (destruct A => //= /andP[/eqP->->]; split; auto).
+    by move=> []; destruct A => -[]// _ ->->//; rewrite eqxx.
+  Qed.
+
+  (* Print resetR'. *)
+
+  Lemma resetR'P L1 L2 B B' R1 R2:
+    resetR' (And L1 B R1) (And L2 B' R2) <-> 
+      if L1 == L2 then R1 == R2 else disj_tree L1 L2 && resetR' R1 R2.
+  Proof. move=> //=. Qed.
+
+  Lemma resetR'_refl A: base_and A -> resetR' A A.
+  Proof. elim: A => //=-[]//=p c _ ?? B HB /andP[/eqP<-]; rewrite eqxx//. Qed.
+
+  Lemma resetR_refl A: base_and A -> resetR A A.
+  Proof. move=> H; rewrite/resetR resetR'_refl//base_and_is_ko//. Qed.
+
+  Lemma step_Exp_CutF s A r:
+    step u s A = r -> get_tree r <> CutS.
+  Proof.
+    move=> <-{r}.
+    case: A => //=.
+    - move=> p c; rewrite/big_or; case: F => [|[]]//.
+    - move=> A sm B; case: ifP; case: step => //.
+    - move=> A B0 B; case: step => // A'; case: step => //.
+  Qed.
+
+  Lemma step_Exp_CallF s A r:
+    step u s A = r -> not (is_call (get_tree r)).
+  Proof.
+    move=> <-{r}.
+    case: A => //=.
+    - move=> p c; rewrite/big_or; case: F => [|[]]//.
+    - move=> A sm B; case: ifP; case: step => //.
+    - move=> A B0 B; case: step => // A'; case: step => //.
+  Qed.
+
+
+  (* Lemma disj_tree_callS_big_or p s c:
+    disj_tree (CallS p c) (big_or u p s c).
+  Admitted. *)
+
+  (* Lemma resetR_base_and s B0 B C:
+    base_and B0 -> 
+    (*valid_tree B ->*) resetR B0 B -> step u s B = C -> resetR B0 (get_tree C).
+  Proof.
+    rewrite/resetR => HB + <-.
+    rewrite base_and_is_ko//=.
+    elim: B s B0 HB => //[p c s []|_ []|?????? []|]//.
+    move=> A HA B0 HB0 B HB s []// L _ R /base_and_AndP[[]+ -> bR];
+    case: L => //.
+      move=> _.
+      move=> /resetR'P; case:eqP => H; subst.
+        move=> /eqP ?; subst => /=.
+        by rewrite disj_tree_baseL//resetR'_refl.
+      move=> /andP[_]/= H1.
+      have:= HA s.
+      case eA: step => //=[A'|A'|A'|A'];
+      only 1, 2, 3: (move=> {}HA; case: eqP => //?; subst; (try by have:= step_Exp_CutF eA); rewrite disj_tree_baseL//=).
+      move=>{}HA.
+      have [? sA]:= expand_solved_same _ eA; subst.
+      have:= HB (get_substS s A') _ bR H1; case eB: step => //=[B'|B'|B'|B']->;
+      rewrite disj_tree_baseL//=; case: eqP; auto.
+      destruct A' => //=; case: ifP => //.
+    move=> p c _ /resetR'P; case: eqP => H.
+      move=> /eqP?; subst => /=; case: ifP => //= _.
+      rewrite resetR'_refl//andbT disj_tree_callS_big_or//.
+    move=> /andP[H1 HR]/=.
+    have:= HA s.
+    case eA: step => //=[A'|A'|A'|A'];
+    only 1, 2, 3: (move=> {}HA; case: eqP => //?; subst; (try by have:= step_Exp_CallF eA); rewrite HR (disj_tree_stepR eA)//).
+    move=> {}HA.
+    have [? sA]:= expand_solved_same _ eA; subst.
+    have:= HB (get_substS s A') _ bR HR; case eB: step => //=[B'|B'|B'|B']->;
+    case: eqP; auto; rewrite?H1//.
+      by destruct A' => //=; case: ifP => //.
+    rewrite disj_tree_cutlR//.
+  Qed.
+
+  Lemma resetR_step s B0 B C:
+    bbAnd B0 -> resetR B0 B -> step u s B = C -> resetR B0 (get_tree C).
+  Proof.
+    move=> /orP[]; last by move=> + _ => /resetR_base_and_ko ->//.
+    apply: resetR_base_and.
+  Qed. *)
 
   Lemma valid_tree_expand {s A r}:
     valid_tree A -> step u s A = r -> valid_tree (get_tree r).
@@ -338,31 +581,25 @@ Section valid_tree.
     elim: A s => //; try by move=> s r // *; subst.
     + by move=> ? ? ?? *;subst => //=; rewrite valid_tree_big_or.
     + move=> A IHA s B IHB s1/=.
-      case:ifP => //[dA vB|dA/andP[vA bB]].
+      case:ifP => //[dA /andP[dAB vB]|dA/and3P[dAB vA bB]].
         rewrite get_tree_Or/=dA IHB//.
+        rewrite disj_tree_commE (disj_tree_step erefl)//disj_tree_commE//.
       have /= := IHA s1 vA.
-      case X: step => //= H; rewrite (step_not_dead _ dA X) H//bbOr_cutr//.
+      case X: step => //=[A'|A'|A'|A'] H; 
+      rewrite !(step_not_dead _ dA X, H,bB,bbOr_cutr,disj_tree_cutrR,disj_tree_step X)//=.
     + move=> A HA B0 _ B HB s1 /=/and4P[vA ++ CC].
       case: ifP => [sA vB /= bB0 | sA /eqP->]/=.
         rewrite succes_is_solved//=.
         have {HB} := HB (get_substS s1 A) vB.
-        case X: step => //[C|C|C|C]/=vC; cycle 1; [|by rewrite sA vA vC /=bB0/=(check_cut_step _ X)..].
-        by rewrite success_cut sA/= valid_tree_cut//vC bbAnd_cutr//check_cut_cutrR.
+        case X: step => //[C|C|C|C]/=vC; cycle 1; [|by rewrite sA vA vC /=bB0/=(check_cut_step _ X isT) CC..].
+        rewrite success_cut sA/= valid_tree_cut//vC bbAnd_cutr//check_cut_cutrR//.
       case: ifP => [fA bB|fA bB].
         by rewrite failed_expand//= vA sA eqxx bB/=fA// check_cut_refl.
       have:= HA s1 vA.
       case X: step => //[A'|A'|A'|A']/=vA'; last first;
-       [|by rewrite //vA' base_and_valid///bbAnd bB eqxx !if_same//check_cut_refl..].
+       [|by rewrite //vA' base_and_valid///bbAnd bB eqxx !if_same//check_cut_refl// if_same..].
       have [? sA']:= expand_solved_same _ X; subst.
       congruence.
-  Qed.
-
-  Lemma valid_tree_big_or_aux {pr s l} : valid_tree (big_or_aux pr s l).
-  Proof.
-    elim: l s => [|[]] //=.
-    + move=> s; rewrite valid_tree_big_and // full_expanded_big_and.
-    + move=> _ r l IH s.
-      rewrite valid_tree_big_and bbOr_big_or_aux IH if_same//.
   Qed.
 
   Lemma next_alt_aux_base_and {A}: base_and A -> next_alt false A = Some (A).
@@ -374,20 +611,19 @@ Section valid_tree.
   Lemma next_alt_aux_base_and_ko {A} b: base_and_ko A -> next_alt b A = None.
   Proof. elim: A => //=; move=>/=[]//p a _ B0 HB0 B HB s/andP[/eqP->bB]/=. Qed.
 
-  Lemma base_and_failed {A}: base_and A -> failed A = false.
-  Proof. elim: A => //=-[]//=p a _ A HA B HB /andP[]//. Qed.
-
   Lemma base_and_is_dead {A}: base_and A -> is_dead A = false.
   Proof. move=>/base_and_failed; apply: contraFF is_dead_failed. Qed.
-
-  Lemma base_and_ko_is_ko {A}: base_and_ko A -> is_ko A.
-  Proof. elim: A => //=-[]//. Qed.
 
   Lemma base_and_ko_is_dead {A}: base_and_ko A -> is_dead A = false.
   Proof. case: A => //-[]//. Qed.
 
   Lemma base_or_failed {A}: base_or_aux A -> failed A = false.
-  Proof. elim: A => //=-[]//=[]//. Qed.
+  Proof. 
+    elim: A=> //=.
+    - move=> A HA s B HB /and3P[dA bA bB]; case: ifP => _; auto.
+      by apply: base_and_failed.
+    - move=> []//=.
+  Qed.
 
   Lemma base_or_is_dead {A}: base_or_aux A -> is_dead A = false.
   Proof. move=>/base_or_failed; apply: contraFF is_dead_failed. Qed.
@@ -424,7 +660,7 @@ Section valid_tree.
   Lemma next_alt_aux_base_or_none {A}: base_or_aux A -> next_alt false A = None -> A = Bot.
   Proof. 
     elim: A => //. 
-    - move=> A HA s B HB /= /andP[bA bB].
+    - move=> A HA s B HB /= /and3P[dAB bA bB].
       rewrite base_and_dead//next_alt_aux_base_and//.
     - move=>A; case: A => //[p a|] _ B0 HB0 B HB/andP[/eqP->bB]/=;
       rewrite next_alt_aux_base_and//. 
@@ -466,6 +702,74 @@ Section valid_tree.
     valid_tree A -> next_alt b A = Some B -> check_cut B B0 = check_cut A B0.
   Proof. move=> vA nA; rewrite /check_cut (next_alt_keep_cut vA nA)//. Qed.
 
+  Lemma disj_tree_next_alt A B D b:
+    disj_tree A D -> next_alt b A = Some B -> disj_tree B D.
+  Proof.
+    elim: A B b => //=.
+    - move=> B []// _ [<-]//.
+    - move=> p c B// _ H [<-]//.
+    - move=> B _ H [<-]//.
+    - move=> A HA s B HB C b /disj_tree_Or[dA dB].
+      case nA: next_alt => [A'|].
+        by move=> [<-]; apply/disj_tree_Or; rewrite dB (HA _ _ dA nA).
+      case nB: next_alt => [B'|]//[<-].
+      apply/disj_tree_Or; rewrite (HB _ _ dB nB).
+      case:ifP; split; rewrite //disj_tree_deadL//.
+    - move=> A HA B0 HB0 B HB C b /disj_tree_And[dA dB0 dB].
+      case:ifP => fA.
+        case nA: next_alt => [A'|]//.
+        case nB0: next_alt => [B0'|]//[<-].
+        by apply/disj_tree_And; split; rewrite //(HA _ _ _ nA,HB0 _ _ _ nB0).
+      case: ifP => sA; last by move=> [<-]; apply/disj_tree_And; split.
+      case nB: next_alt => [B'|].
+        by move=>[<-]; apply/disj_tree_And; split; rewrite//(HB _ _ _ nB).
+      case nA: next_alt => [A'|]//.
+      case nB0: next_alt => [B0'|]//[<-].
+      by apply/disj_tree_And; split; rewrite //(HA _ _ _ nA,HB0 _ _ _ nB0).
+  Qed.
+
+  Lemma disj_tree_next_altR A B D b:
+    disj_tree D A -> next_alt b A = Some B -> disj_tree D B.
+  Proof. by move=> /disj_tree_comm dA /(disj_tree_next_alt dA)/disj_tree_comm. Qed.
+
+  Lemma resetR_next_alt A B B0 b:
+    bbAnd B0 ->
+    valid_tree A -> next_alt b A = Some B -> 
+    resetR B0 A -> resetR B0 B.
+  Proof.
+    rewrite/resetR.
+    move=> /orP[]bB; last by rewrite base_and_ko_is_ko//.
+    rewrite base_and_is_ko//=.
+    elim: A B B0 b bB => //=.
+    - move=> B []//[]// _ _ [<-]//.
+    - move=> p c B []//=.
+    - move=> B []//.
+    - move=> A HA s B HB C []//.
+    - move=> A HA B0 HB0 B HB C []// L _ R b /base_and_AndP[H -> bR] /and4P[vA ++ cK] + /resetR'P.
+      case:ifP => [sA vB/= bB0|sA/eqP->{B0 HB0 cK}]/=.
+        rewrite success_failed//=.
+        case nB: next_alt => [B'|].
+          move=> [<-]; case: eqP => H1; subst.
+            by move: H => []; destruct A => //.
+          move=> /andP[->]; apply: HB; eauto.
+        case nA: next_alt => //=[A'].
+        case nB0: next_alt => //=[B0'][<-].
+        case: eqP => H1; subst.
+          by move: H => []; destruct A => //.
+        move=> /andP[H2 H3].
+        case: eqP => H4; subst.
+           (*to satisfy nA A should be == A': contradicts H1*)
+          admit.
+        rewrite (disj_tree_next_altR H2 nA)/=.
+        move/orP: bB0 => []bB; last first.
+          by rewrite (is_ko_next_alt _ (base_and_ko_is_ko bB)) in nB0.
+        move: nB0; rewrite next_alt_aux_base_and//.
+        move=> [<-]{B0'}.
+        (* move/orP: rB; rewrite base_and_is_ko// => -[]//rR'. *)
+        (* Print resetR'. *)
+
+  Abort.
+
   Lemma valid_tree_next_alt {A B b}: 
     valid_tree A -> next_alt b A = Some (B) 
     -> valid_tree B.
@@ -475,19 +779,19 @@ Section valid_tree.
     + move=> p c B _ _ [<-]//.
     + move=> B _ _ [<-]//.
     + move=> A HA s B HB  C b/=.
-      case: ifP => //[dA vB|dA /andP[vA bB]].
+      case: ifP => [dA /andP[dAB vB]|dA /and3P[dAB vA bB]].
         rewrite is_dead_next_alt//.
         case X: next_alt => //[D] [<-]/=.
-        rewrite dA (HB _ _ vB X)//.
+        by rewrite dA (HB _ _ vB X)// (disj_tree_next_altR _ X).
       case X: next_alt => [D|].
-        move=>[<-]/=; rewrite bbOr_valid// bB (HA _ _ vA X) if_same//.
-      case Y: next_alt => [D|]//[<-]/=; rewrite is_dead_dead (HB _ _ _ Y)//bbOr_valid//.
+        by move=>[<-]/=; rewrite bbOr_valid// bB (HA _ _ vA X) if_same (disj_tree_next_alt dAB X).
+      by case Y: next_alt => [D|]//[<-]/=; rewrite is_dead_dead disj_tree_deadL (HB _ _ _ Y)//bbOr_valid.
     + move=> A HA B0 HB0 B HB  C b /=/and4P[vA ++ CC].
-      case: ifP => /=[sA vB bB0|sA /eqP?]; subst.
+      case: ifP => /=[sA vB  bB0|sA /eqP?]; subst.
         rewrite success_failed//.
         case X: next_alt => [D|].
           move=>[<-]/=; rewrite vA sA/= (HB _ _ vB X)//bB0/=.
-          by rewrite (next_alt_check_cut vB X).
+          by rewrite (next_alt_check_cut vB X) CC.
         case Y: next_alt => //=[A'].
         move: bB0 => /orPT[]/[dup]bB; last first.
           move=> /(next_alt_aux_base_and_ko false) -> //.
